More wip

CoqOfRust/revm/revm_interpreter/instructions/simulate/arithmetic.v
@@ -10,40 +10,157 @@ Require Import revm.revm_interpreter.links.interpreter_types.
 Definition make_ref {A : Set} `{Link A} {kind : Pointer.Kind.t} (index : nat) : Ref.t kind A :=
   {| Ref.core := Ref.Core.Mutable (A := A) index [] φ Some (fun _ => Some) |}.
 
+Module RefStub.
+  Record t {A Sub_A : Set} `{Link A} `{Link Sub_A} : Set := {
+    path : Pointer.Path.t;
+    (* We suppose the pointer is valid (no [option] type for the [projection] and [injection]
+       functions) *)
+    projection : A -> Sub_A;
+    injection : A -> Sub_A -> A;
+  }.
+  Arguments t _ _ {_ _}.
+
+  Definition apply_core {A Sub_A : Set} `{Link A} `{Link Sub_A}
+      (ref_core : Ref.Core.t A)
+      (stub : t A Sub_A) :
+      Ref.Core.t Sub_A.
+  Proof.
+    destruct ref_core as [| ? ? address path big_to_value projection injection].
+    { (* Immediate *)
+      exact (
+        Ref.Core.Immediate (
+          match value with
+          | Some a => Some (stub.(projection) a)
+          | None => None
+          end
+        )
+      ).
+    }
+    { (* Mutable *)
+      exact (
+        Ref.Core.Mutable
+          address
+          (path ++ stub.(RefStub.path))
+          big_to_value
+          (fun big_a =>
+            match projection big_a with
+            | Some a => Some (stub.(RefStub.projection) a)
+            | None => None
+            end
+          )
+          (fun big_a new_sub_a =>
+            match projection big_a with
+            | Some a =>
+              let new_a := stub.(RefStub.injection) a new_sub_a in
+              injection big_a new_a
+            | None => None
+            end
+          )
+      ).
+    }
+  Defined.
+
+  Definition apply {A Sub_A : Set} `{Link A} `{Link Sub_A}
+      {kind_source kind_target : Pointer.Kind.t}
+      (ref : Ref.t kind_source A)
+      (stub : t A Sub_A) :
+      Ref.t kind_target Sub_A :=
+    {| Ref.core := apply_core ref.(Ref.core) stub |}.
+End RefStub.
+
 Module Stack.
-  Class C (WIRE_types : InterpreterTypes.Types.t) : Set := {
+  (* Definition t : Set :=
+    list aliases.U256.t. *)
+
+  (* Fixpoint popn_top (POPN : nat) (stack : t) :
+      option (array.t aliases.U256.t {| Integer.value := Z.of_nat POPN |}) * t :=
+    match POPN, stack with
+    | O, [] => (Some {| array.value := [] |}, stack)
+    | S POPN, [] => (None, stack)
+    | S POPN, x :: xs =>
+        match popn_top POPN xs with
+        | (Some a, stack') => (Some {| array.value := x:: a.(array.value) |}, stack')
+        | (None, _) => (None, stack)
+        end
+    | _, _ => (None, stack)
+    end. *)
+
+  (* Definition pop2_top (stack : t) : option (array.t aliases.U256.t {| Integer.value := 2 |}) * t :=
+    match stack with
+    | x1 :: x2 :: rest => (Some {| array.value := [x1; x2] |}, rest)
+    | _ => (None, stack)
+    end. *)
+
+  Class C
+      (WIRE_types : InterpreterTypes.Types.t) `{InterpreterTypes.Types.AreLinks WIRE_types} :
+      Type := {
     popn_top :
       forall
         (POPN : Usize.t)
         (self : WIRE_types.(InterpreterTypes.Types.Stack)),
-      (option (array.t aliases.U256.t POPN * Z)) *
+      option (
+        array.t aliases.U256.t POPN *
+        RefStub.t WIRE_types.(InterpreterTypes.Types.Stack) aliases.U256.t
+      ) *
       WIRE_types.(InterpreterTypes.Types.Stack);
   }.
 
   Module Eq.
-    Record t
-        {WIRE : Set} `{Link WIRE}
-        {WIRE_types : InterpreterTypes.Types.t} `{InterpreterTypes.Types.AreLinks WIRE_types}
+    Class t
+        (WIRE : Set) (WIRE_types : InterpreterTypes.Types.t)
+        `{Link WIRE} `{InterpreterTypes.Types.AreLinks WIRE_types}
         (run_InterpreterTypes_for_WIRE : InterpreterTypes.Run WIRE WIRE_types)
         (I : C WIRE_types) :
         Prop := {
       popn_top
-          (Stack : list Set) (stack : Stack.to_Set Stack)
-          (POPN : Usize.t)
-          (self : WIRE_types.(InterpreterTypes.Types.Stack)) :
-        let ref_self := make_ref 0 in
+          (Stack : list Set)
+          (interpreter : Interpreter.t WIRE WIRE_types)
+          (stack_rest : Stack.to_Set Stack)
+          (POPN : Usize.t) :
+        let ref_interpreter : Ref.t Pointer.Kind.MutRef _ := make_ref 0 in
+        let ref_self := {| Ref.core :=
+          SubPointer.Runner.apply
+            ref_interpreter.(Ref.core)
+            Interpreter.SubPointer.get_stack
+        |} in
         {{
-          StackM.eval_f (Stack := WIRE_types.(InterpreterTypes.Types.Stack) :: Stack)
+          StackM.eval_f (Stack := Interpreter.t WIRE WIRE_types :: Stack)
             (run_InterpreterTypes_for_WIRE.(InterpreterTypes.run_StackTrait_for_Stack).(StackTrait.popn_top).(TraitMethod.run)
               POPN
               ref_self
             )
-            (self, stack) 🌲
-          (Output.Success None, (self, stack))
+            (interpreter, stack_rest) 🌲
+          let (result, self) := I.(popn_top) POPN interpreter.(Interpreter.stack) in
+          let result :=
+            match result with
+            | Some (a, stub) => Some (a, RefStub.apply ref_self stub)
+            | None => None
+            end in
+          (Output.Success result, (interpreter <| Interpreter.stack := self |>, stack_rest))
         }};
     }.
   End Eq.
 End Stack.
+
+Parameter wrapping_add :
+  forall {BITS LIMBS : Usize.t} (x1 x2 : lib.Uint.t BITS LIMBS),
+  lib.Uint.t BITS LIMBS.
+
+Lemma wrapping_add_eq (BITS LIMBS : Usize.t) (x1 x2 : lib.Uint.t BITS LIMBS) :
+  links.M.evaluate (add.Impl_Uint.run_wrapping_add BITS LIMBS x1 x2).(Run.run_f) =
+  links.M.LowM.Pure (Output.Success (wrapping_add x1 x2)).
+Admitted.
+
+(* Lemma wrapping_add_eq
+    {Stack : Stack.t} (stack : Stack.to_Set Stack)
+    (BITS LIMBS : Usize.t) (x1 x2 : lib.Uint.t BITS LIMBS) :
+  {{
+    StackM.eval_f (Stack := Stack)
+      (add.Impl_Uint.run_wrapping_add BITS LIMBS x1 x2)
+      stack 🌲
+    (Output.Success (wrapping_add x1 x2), stack)
+  }}.
+Admitted. *)
 
 (*
   {{StackM.eval
@@ -90,24 +207,68 @@ Lemma add_eq
     {WIRE_types : InterpreterTypes.Types.t} `{InterpreterTypes.Types.AreLinks WIRE_types}
     {H_types : Host.Types.t} `{Host.Types.AreLinks H_types}
     (run_InterpreterTypes_for_WIRE : InterpreterTypes.Run WIRE WIRE_types)
+    (IStack : Stack.C WIRE_types)
+    (StackEq : Stack.Eq.t WIRE WIRE_types run_InterpreterTypes_for_WIRE IStack)
     (interpreter : Interpreter.t WIRE WIRE_types)
     (_host : H) :
   let ref_interpreter := make_ref 0 in
   let ref_host := make_ref 1 in
   {{
-    StackM.eval_f (Stack := [_; _]) (run_add run_InterpreterTypes_for_WIRE ref_interpreter ref_host) (interpreter, _host) 🌲
-    (Output.Success tt, (interpreter, _host))
+    StackM.eval_f (Stack := [_; _]) (run_add run_InterpreterTypes_for_WIRE ref_interpreter ref_host) (interpreter, (_host, tt)) 🌲
+    (Output.Success tt, (interpreter, (_host, tt)))
   }}.
 Proof.
   intros.
+  destruct StackEq.
   Time unfold run_add, StackM.eval_f, StackM.eval, evaluate.
   Time hnf.
   Time cbn.
   Time get_can_access.
   Time cbn.
   Time eapply Run.Call. {
-    Print Output.t.
+    apply popn_top.
   }
-  Show.
+  Time destruct IStack.(Stack.popn_top) as [[[? ?]|] ?].
+  { Time get_can_access.
+    Time cbn.
+    Time destruct t0.(array.value).
+    { Time cbn.
+      (* Show. *)
+      admit.
+    }
+    { Time cbn.
+      Time repeat get_can_access.
+      Time eapply Run.Call. {
+        rewrite wrapping_add_eq.
+        apply Run.Pure.
+      }
+      destruct wrapping_add.
+      Time cbn.
+      Time repeat get_can_access.
+      Show.
+
+    }
+  Time unshelve eapply Run.GetCanAccess. {
+      Time cbn.
+      match goal with
+      | |- Stack.CanAccess.t ?Stack (Ref.Core.Mutable ?index _ _ _ ?injection) =>
+        apply (Stack.CanAccess.Mutable Stack index _ _ _ injection)
+      end.
+      Show.
+      
+    }
+    Time match goal with
+    | |- Run.t _ ?e =>
+      let e' := fresh "e'" in
+      let e' := eval hnf in e in
+      change e with e'
+    end.
+    (* Time get_can_access. *)
+    Time cbn.
+    Show.
+
+  }
+  (* Time cbn. *)
+  (* Show. *)
   
 Qed.
